progs/VSUpile/verif_stdlib.v
@@ -6,8 +6,10 @@ Require Import spec_stdlib.
 
 Instance CompSpecs : compspecs. make_compspecs prog. Defined.
 
-Section MallocFree_VSU.
-Variable M: MallocFreeAPD.
+Parameter M: MallocFreeAPD.
+
+Axiom mem_mgr_rep: forall gv, emp |-- mem_mgr M gv.
+
 Parameter body_malloc:
  forall {Espec: OracleKind} {cs: compspecs} ,
    VST.floyd.library.body_lemma_of_funspec EF_malloc (snd (malloc_spec' M)).
@@ -39,6 +41,9 @@ Definition placeholder_spec :=
   Definition MFVprog : varspecs. mk_varspecs prog. Defined.
   Definition MFGprog: funspecs := MF_imported_specs ++ MF_internal_specs.
 
+  Lemma MF_Init: VSU_initializer prog (mem_mgr M).
+  Proof. InitGPred_tac. apply mem_mgr_rep. Qed.
+
 Lemma body_placeholder: semax_body MFVprog MFGprog f_placeholder placeholder_spec.
 Proof.
 start_function.
@@ -64,71 +69,20 @@ Proof.
  if_tac. rewrite H; entailer!.
  renormalize. entailer!.
 Qed.
-(*Existing Instance NullExtension.Espec.*)
-(*
-Lemma tcret_malloc: 
-tcret_proof (tptr tvoid) (rmaps.ConstType (Z * globals))
-  (fun (_ : list Type) (x : Z * globals) =>
-   let (n, gv) := x in
-   (EX p : val,
-    PROP ( )
-    LOCAL (temp ret_temp p)
-    SEP (mem_mgr gv;
-    if @eq_dec val Memory.EqDec_val p nullval
-    then @emp mpred Nveric Sveric
-    else malloc_token' Ews n p * memory_block Ews n p))%assert).
-Proof.
-red; intros.
-destruct x.
- rewrite exp_unfold. Intros p.
- rewrite <- insert_local.
- rewrite lower_andp.
- red in H. simpl in H. destruct ret; try contradiction. clear H.
- apply derives_extract_prop; intro.
- destruct H; unfold_lift in H.  rewrite retval_ext_rval in H. simpl in H. subst p.
- unfold_lift in H0. 
- if_tac. rewrite H; entailer!.
- renormalize. entailer!. simpl. auto.
-Qed.
-Lemma tcret_free:
-   tcret_proof tvoid (rmaps.ConstType (Z * val * globals))
-  (fun (_ : list Type) (x : Z * val * globals) =>
-   let (p0, gv) := x in
-   let (_, _) := p0 in PROP ( )  LOCAL ()  SEP (mem_mgr gv)).
-Proof.
-hnf; intros; normalize.
-Qed.
 
 
-Lemma tcret_exit: 
-  tcret_proof tvoid (rmaps.ConstType Z)
-  (fun (_ : list Type) (_ : Z) => PROP (False)  LOCAL ()  SEP ()).
-Proof.
-hnf; intros; normalize.
-Qed.*)
+Definition MF_E : funspecs := MF_ASI.
 
-(*Maybe we should add the specs for malloc, free, exit, also into the E argument?
-  Maybe the type of the E argument should not be funspecs, but 
-   external_function * funspec)?*)
-
-  Definition MF_E : funspecs := MF_ASI.
-
-  Definition MallocFreeComponent: @Component NullExtension.Espec MFVprog CompSpecs 
-      (*nil*)MF_E MF_imported_specs prog MF_ASI emp MF_internal_specs.
+Definition MallocFreeVSU: @VSU NullExtension.Espec
+         MF_E MF_imported_specs ltac:(QPprog prog) MF_ASI (mem_mgr M).
   Proof. 
-    mkComponent. 
-    - clear; solve_SF_external (@body_malloc NullExtension.Espec CompSpecs). 
+    mkVSU prog MF_internal_specs.
+    - solve_SF_external (@body_malloc NullExtension.Espec CompSpecs). 
       Intros. eapply derives_trans.
       apply (semax_func_cons_malloc_aux gv gx ret n).
       destruct ret; simpl; trivial.
-    - clear; solve_SF_external (@body_free NullExtension.Espec CompSpecs).
-    - clear; solve_SF_external (@body_exit NullExtension.Espec).
-    - clear; solve_SF_internal body_placeholder.
-Time  Qed. (*2.5s*)
-
-Definition MallocFreeVSU: @VSU NullExtension.Espec MFVprog CompSpecs 
-      (*nil*)MF_E MF_imported_specs prog MF_ASI emp.
-  Proof. eexists; apply MallocFreeComponent. Qed.
-End MallocFree_VSU.
-
-
+    - solve_SF_external (@body_exit NullExtension.Espec).
+    - solve_SF_internal body_placeholder.
+    - solve_SF_external (@body_free NullExtension.Espec CompSpecs).
+    - apply MF_Init.
+Qed.
