progs/VSUpile/verif_triang.v
@@ -53,14 +53,12 @@ reflexivity.
 simpl. congruence.
 Qed.
 
-  Definition TriangComponent: @Component NullExtension.Espec TriangVprog _ 
-      nil triang_imported_specs prog (TriangASI M) emp triang_internal_specs.
-  Proof. 
-    mkComponent. 
+ 
+Definition TriangVSU: @VSU NullExtension.Espec
+      nil triang_imported_specs ltac:(QPprog prog) (TriangASI M) emp.
+Proof.
+  mkVSU prog triang_internal_specs.
     + solve_SF_internal body_Triang_nth.
-  Qed.
+Qed.
 
-Definition TriangVSU: @VSU NullExtension.Espec TriangVprog _ 
-      nil triang_imported_specs prog (TriangASI M) emp.
-  Proof. eexists; apply TriangComponent. Qed.
 End Triang_VSU.
